made a bit of a mess

src/Bedrock/Field/Synthesis/Examples/redc.v
@@ -2,29 +2,33 @@ Require Import bedrock2.NotationsCustomEntry.
 
 Import Syntax BinInt String List.ListNotations.
 Local Open Scope string_scope. Local Open Scope Z_scope. Local Open Scope list_scope.
+From coqutil.Word Require Import Interface Properties.
 
 From bedrock2 Require Import WeakestPrecondition WeakestPreconditionProperties
   Syntax Semantics BasicC64Semantics ProgramLogic Scalars Array Loops ZnWords.
 From bedrock2.Map Require Import Separation SeparationLogic.
 Require Import coqutil.Map.Interface.
-From coqutil.Word Require Import Interface Properties.
+
 
 From coqutil.Tactics Require Import Tactics letexists eabstract.
 Require Import Coq.ZArith.ZArith.
 From coqutil.Z Require Import div_mod_to_equations Lia.
+Require Import Coq.Program.Tactics.
 
 Require Import Crypto.Arithmetic.WordByWordMontgomery.
+Import Markers.
+
 
 Section WithParameters.
   
   Import List.
   Import WordByWordMontgomery.
   
-  Context {prime: Z} (r := 32) {ri : Z}.
+  Context {prime: Z} (r := 64) {ri : Z}.
   Context {ri_correct: (ri * r) mod prime = 1}.
   (* prime is the modulus; r is the word size; ri is the inverse of r mod prime *)
-  Context {word: word.word r} {mem: map.map word Byte.byte}.
-  Context {word_ok: word.ok word} {mem_ok: map.ok mem}.
+  (*Context {word: word.word r} {mem: map.map word Byte.byte}.
+  Context {word_ok: word.ok word} {mem_ok: map.ok mem}.*)
   
   Local Notation "m =* P" := ((P%sep) m) (at level 70, only parsing) (* experiment*).
 
@@ -35,17 +39,17 @@ Section WithParameters.
   Instance spec_of_redc_alt : spec_of "redc_alt" :=
     fnspec! "redc_alt" Astart Bstart Sstart len / A (aval: Z) B (bval: Z) S Ra Rb R,
     { requires t m :=
-        m =* array scalar (word.of_Z 4) Astart A * Ra /\
-        m =* array scalar (word.of_Z 4) Bstart B * Rb /\
-        m =* array scalar (word.of_Z 4) Sstart S * R /\
+        m =* array scalar (word.of_Z 8) Astart A * Ra /\
+        m =* array scalar (word.of_Z 8) Bstart B * Rb /\
+        m =* array scalar (word.of_Z 8) Sstart S * R /\
         word.unsigned len = Z.of_nat (List.length A)  /\
         word.unsigned len = Z.of_nat (List.length B)  /\
         word.unsigned len = Z.of_nat (List.length S) /\
         @eval r (Z.to_nat (word.unsigned len)) (List.map word.unsigned A) = aval /\ 
         @eval r (Z.to_nat (word.unsigned len)) (List.map word.unsigned B) = bval;                                       
       ensures t' m' :=  t=t' /\ exists S', 
-          m' =* array scalar (word.of_Z 4) Sstart S' * R /\
-          ( aval * bval * ri ) mod prime =
+          m' =* array scalar (word.of_Z 8) Sstart S' * R /\
+          ( aval * bval * ri^(word.unsigned len) ) mod prime =
             @eval r (Z.to_nat (word.unsigned len)) (List.map word.unsigned S') mod prime
     }.
 
@@ -55,69 +59,55 @@ Section WithParameters.
   Instance spec_of_redc_step : spec_of "redc_step" := 
     fnspec! "redc_step" a Bstart Sstart len / B (bval: Z) S (sval: Z) R Rb,
       { requires t m :=
-          m =* array scalar (word.of_Z 4) Bstart B * Rb /\
-          m =* array scalar (word.of_Z 4) Sstart S * R /\
+          m =* array scalar (word.of_Z 8) Bstart B * Rb /\
+          m =* array scalar (word.of_Z 8) Sstart S * R /\
           word.unsigned len = Z.of_nat (List.length B) /\
           word.unsigned len = Z.of_nat (List.length S) /\
           @eval r (Z.to_nat (word.unsigned len)) (List.map word.unsigned B) = bval /\
           @eval r (Z.to_nat (word.unsigned len)) (List.map word.unsigned S) = sval;
         ensures t' m' := t=t' /\ exists S',
-            m' =* array scalar (word.of_Z 4) Sstart S' * R /\
+            m' =* array scalar (word.of_Z 8) Sstart S' * R /\
               ((word.unsigned a) * bval + sval) * ri mod prime =
                 @eval r (Z.to_nat (word.unsigned len)) (List.map word.unsigned S') mod prime
-      }.  
-  
+      }.
+
   Definition redc_alt : func :=
     let redc_step : String.string := "redc_step" in 
     ("redc_alt", (["Astart"; "Bstart"; "Sstart"; "len"], [], bedrock_func_body:(
     i = $0;
     while (i < len) { 
-         store4(Sstart + $4*i, $0);
-         i = i << $1          
+         store(Sstart + $8*i, $0);
+         i = i + $1          
       };
     i = $0;       
     while (i < len) {
-         redc_step ( load4(Astart + $4*i), Bstart, Sstart, len ); 
-          i = i << $1
+         redc_step ( load(Astart + $8*i), Bstart, Sstart, len ); 
+          i = i + $1
       }
     ))).
 
   Require Import Coq.Lists.List.
-(*
-  Let wordy_zero (n : word) :=
-        repeat (@word.of_Z _ word 0) (Z.to_nat (word.unsigned n)). *)
 
-  
-  Theorem redc_alt_ok :
+  Let zeros (n: Z) :=
+        repeat (@word.of_Z _ word 0) (Z.to_nat n).
+
+ Theorem redc_alt_ok :
       program_logic_goal_for_function! redc_alt.
     Proof.
-      repeat straightline. 
-
+      repeat straightline.
+      (*after the first loop, our output array is full of zeros*)
       refine ( tailrec (HList.polymorphic_list.cons _ (HList.polymorphic_list.cons _ (HList.polymorphic_list.cons _ (HList.polymorphic_list.cons _ (HList.polymorphic_list.cons _ (HList.polymorphic_list.cons _ (HList.polymorphic_list.cons _ (HList.polymorphic_list.cons _ HList.polymorphic_list.nil))))))))
                ("Astart":: "Bstart" :: "Sstart" :: "len" :: "i" :: nil)
                (fun l A aval B bval S Ra Rb R t m Astart Bstart Sstart len i => PrimitivePair.pair.mk
-                                    (m =* array scalar (word.of_Z 4) Astart A * Ra /\
-                                     m =* array scalar (word.of_Z 4) Bstart B * Rb /\
-                                     m =* array scalar (word.of_Z 4) Sstart S * R /\
-                                     word.unsigned len = Z.of_nat (List.length A)  /\
-                                     word.unsigned len = Z.of_nat (List.length B)  /\
-                                     word.unsigned len = Z.of_nat (List.length S) /\
-                                     @eval r (Z.to_nat (word.unsigned len)) (List.map word.unsigned A) = aval /\ 
-                                     @eval r (Z.to_nat (word.unsigned len)) (List.map word.unsigned B) = bval /\
-                                     @eval r (Z.to_nat (word.unsigned i)) (List.map word.unsigned S) = 0)
+                                    (m =* array scalar (word.of_Z 8) (word.add Sstart (word.mul (word.of_Z 8) i)) S * R /\
+                                       word.unsigned len - word.unsigned i = Z.of_nat (List.length S) /\
+
+                                       
+                                    l = List.length S ) 
                                     (fun t' m' Astart' Bstart' Sstart' len' i' =>
                                        (
-                                     t = t' /\
-                                     m' =* array scalar (word.of_Z 4) Astart A * Ra /\
-                                     m' =* array scalar (word.of_Z 4) Bstart B * Rb /\
-                                     word.unsigned len = Z.of_nat (List.length A)  /\
-                                     word.unsigned len = Z.of_nat (List.length B)  /\
-                                     @eval r (Z.to_nat (word.unsigned len)) (List.map word.unsigned A) = aval /\ 
-                                     @eval r (Z.to_nat (word.unsigned len)) (List.map word.unsigned B) = bval /\
-                                     exists S',
-                                     m' =* array scalar (word.of_Z 4) Sstart S' * R  /\
-                                     word.unsigned len = Z.of_nat (List.length S') /\
-                                     @eval r (Z.to_nat (word.unsigned len)) (List.map word.unsigned S') = 0
+                                     t = t' /\ Astart = Astart' /\ Bstart = Bstart' /\ Sstart = Sstart' /\ len = len' /\
+                                     m' =* array scalar (word.of_Z 8) (word.add Sstart (word.mul (word.of_Z 8) i)) (zeros (word.unsigned len - word.unsigned i)) * R
                                      )
                                     )
                )
@@ -133,27 +123,384 @@ Section WithParameters.
       
       { repeat straightline. }
       { exact Wf_nat.lt_wf. }
-      { apply O. }
-      { repeat straightline. repeat split; try eauto.}
       { repeat straightline.
-        (* on exit *)
-        2: {
-          repeat split; try assumption.
-          exists x3. repeat split; auto.
-          subst br. destruct (word.ltu x11 x10) eqn: Hi.
-          - inversion H17.
-          - clear H17; cbv [eval] in *.
-            rename x10 into len'; rename x11 into i'.
-
-    Abort.
-    (*
+        assert (Hwords: (word.add Sstart (word.mul (word.of_Z 8) i)) = Sstart).
+        { subst i. rewrite <-  word.ring_morph_mul. rewrite Z.mul_0_r.
+          assert (HstartZ: Sstart = word.of_Z (word.unsigned Sstart)) by (rewrite word.of_Z_unsigned; reflexivity).
+          rewrite HstartZ. rewrite <- word.ring_morph_add. rewrite Z.add_0_r. reflexivity.
         }
-        (*step*)
-       
+        rewrite Hwords. repeat split; try eauto. subst i. rewrite word.unsigned_of_Z_0. rewrite H5. ring. }
+
+      { repeat straightline. eexists. split. { repeat straightline. } repeat straightline. split.
+
+        (*loop exits properly*)
+        2: {
+          repeat straightline; repeat split.
+          rename x3 into S'; rename x9 into Sstart'; rename x10 into len'; rename x11 into i'; rename x6 into R'.
+
+          destruct (word.ltu i' len') eqn: Hbreak; try inversion H10; clear H10.
+          destruct (length S') eqn: HS.
+          (*length cannot be nonzero*)
+          2: { rewrite word.unsigned_ltu in Hbreak. Lia.lia. }
+          (*if length is zero, all arrays are the same*)
+          cbv [Z.of_nat] in H9. rewrite H9; clear H9 Hbreak.
+          apply ListUtil.length0_nil in HS.
+          subst S'. apply H8.
+        }
+
+          
+        (*loop body is good*)
+        repeat straightline.
+        rename x3 into S'; rename x9 into Sstart'; rename x10 into len'; rename x11 into i'; rename x6 into R'.
+        destruct S'.
+        - cbv [length Z.of_nat] in H9. 
+          destruct (word.ltu i' len') eqn: Hbreak; try (rewrite word.unsigned_of_Z_0 in H10; exfalso; apply H10; trivial).
+          rewrite word.unsigned_ltu in Hbreak. Lia.lia. 
+        - cbn [array] in H8. repeat straightline.
+          repeat split; try trivial. exists (S'). repeat split; try trivial. exists ( (scalar (word.add Sstart' (word.mul (word.of_Z 8) i')) (word.of_Z 0)) * R')%sep. exists (length S').
+          repeat split; subst v0 a.
+          all: try (repeat (destruct H12 as [solver H12]; try assumption; clear solver)).
+          + replace (word.mul (word.of_Z 8) i) with (word.add (word.mul (word.of_Z 8) i') (word.of_Z 8)).
+            { rewrite word.add_assoc. apply sep_comm. apply sep_assoc. ecancel_assumption. }
+            { subst i. ring. } 
+          + subst i. 
+            destruct (word.unsigned i' + 1 <? 2^64) eqn: Hisize.
+            2: { assert (2^64 - 1 <= word.unsigned i') by Lia.lia; clear Hisize.
+                 assert (word.unsigned i' < 2^64) by apply word.unsigned_range.
+                 assert (Hi': word.unsigned i' = 2^64 - 1) by Lia.lia; clear H12 H13.
+                 assert (Hlen': word.unsigned len' < 2^64) by apply word.unsigned_range.
+                 assert (Hneg: word.unsigned len' - word.unsigned i' < 1) by Lia.lia; clear Hi' Hlen'.
+                 simpl in H9; simpl in Hneg. rewrite Zpos_P_of_succ_nat in H9.
+                 assert (0 <= (Z.of_nat(length S'))) by apply Zle_0_nat.
+                 Lia.lia.
+            }
+                        
+            rewrite word.unsigned_add. rewrite word.unsigned_of_Z_1. cbv [word.wrap].
+            assert (Hsmall: (word.unsigned i' + 1) mod 2^64 = word.unsigned i' + 1).
+            {  apply Z.mod_small. assert (0 <= word.unsigned i') by apply word.unsigned_range. Lia.lia. }
+            rewrite Hsmall; clear Hisize Hsmall.
+
+            simpl in H9; simpl. rewrite Zpos_P_of_succ_nat in H9.
+            assert (0 <= (Z.of_nat(length S'))) by apply Zle_0_nat.
+            Lia.lia.
+          + subst v.  auto.
+          + assert (Hhead: zeros (word.unsigned len' - word.unsigned i') = word.of_Z 0 :: zeros (word.unsigned len' - word.unsigned i) ).
+            {
+              subst i. 
+            destruct (word.unsigned i' + 1 <? 2^64) eqn: Hisize.
+            2: { assert (2^64 - 1 <= word.unsigned i') by Lia.lia; clear Hisize.
+                 assert (word.unsigned i' < 2^64) by apply word.unsigned_range.
+                 assert (Hi': word.unsigned i' = 2^64 - 1) by Lia.lia; clear H12 H13.
+                 assert (Hlen': word.unsigned len' < 2^64) by apply word.unsigned_range.
+                 assert (Hneg: word.unsigned len' - word.unsigned i' < 1) by Lia.lia; clear Hi' Hlen'.
+                 simpl in H9; simpl in Hneg. rewrite Zpos_P_of_succ_nat in H9.
+                 assert (0 <= (Z.of_nat(length S'))) by apply Zle_0_nat.
+                 Lia.lia.
+            }
+                        
+            rewrite word.unsigned_add. rewrite word.unsigned_of_Z_1. cbv [word.wrap].
+            assert (Hsmall: (word.unsigned i' + 1) mod 2^64 = word.unsigned i' + 1).
+            {  apply Z.mod_small. assert (0 <= word.unsigned i') by apply word.unsigned_range. Lia.lia. }
+            rewrite Hsmall; clear Hisize Hsmall.
+            assert (Hpos: 0 <= word.unsigned len' - (word.unsigned i' + 1)). {
+              simpl in H9; simpl. rewrite Zpos_P_of_succ_nat in H9.
+              assert (0 <= (Z.of_nat(length S'))) by apply Zle_0_nat.
+              Lia.lia.
+            }
+            replace (word.unsigned len' - word.unsigned i') with (Z.succ (word.unsigned len' - (word.unsigned i' + 1)) ) by Lia.lia.
+            cbv [zeros]. rewrite Z2Nat.inj_succ; try assumption. cbn [repeat]. trivial.
+            }
+            rewrite Hhead; clear Hhead.
+            cbn [array]. subst i. 
+            replace (word.add (word.add Sstart' (word.mul (word.of_Z 8) i')) (word.of_Z 8)) with  (word.add Sstart' (word.mul (word.of_Z 8) (word.add i' (word.of_Z 1)))) by ring. ecancel_assumption.
         }
      
-       { }
-    Qed.
-*)
+        {
+          repeat straightline.
+          
+          refine ( tailrec (HList.polymorphic_list.cons _ (HList.polymorphic_list.cons _ (HList.polymorphic_list.cons _ (HList.polymorphic_list.cons _ (HList.polymorphic_list.cons _ (HList.polymorphic_list.cons _ (HList.polymorphic_list.cons _ (HList.polymorphic_list.cons _ HList.polymorphic_list.nil))))))))
+               ("Astart":: "Bstart" :: "Sstart" :: "len" :: "i" :: nil)
+               (fun l A aval B bval S Ra Rb R t m Astart Bstart Sstart len i => PrimitivePair.pair.mk
+                                           (
+                                            (*m =* array scalar (word.of_Z 8) Astart A * Ra /\
+                                            m =* array scalar (word.of_Z 8) Bstart B * Rb /\*)
+                                            m =* array scalar (word.of_Z 8) Sstart S * R /\
+                                            (*word.unsigned len = Z.of_nat (List.length A)  /\
+                                            word.unsigned len = Z.of_nat (List.length B)  /\*)
+                                            word.unsigned len = Z.of_nat (List.length S) /\
+                                            @eval r (Z.to_nat (word.unsigned len)) (List.map word.unsigned A) = aval /\ 
+                                            (*@eval r (Z.to_nat (word.unsigned len)) (List.map word.unsigned B) = bval /\*)
+                                            @eval r (Z.to_nat (word.unsigned len)) (List.map word.unsigned S) mod prime =
+                                            @eval r (Z.to_nat (word.unsigned i)) (List.map word.unsigned A)
+                                            * bval * ri^(word.unsigned i) mod prime /\
+                                             word.unsigned i <= word.unsigned len /\
+                                             l = Z.to_nat (word.unsigned len - word.unsigned i)
+                                           )
+                                    (fun t' m' Astart' Bstart' Sstart' len' i' =>
+                                     (
+                                     t = t' /\ Astart = Astart' /\ Bstart = Bstart' /\ Sstart = Sstart' /\ len = len' /\
+                                     exists S',
+                                       m' =* array scalar (word.of_Z 8) Sstart S' * R /\
+                                       @eval r (Z.to_nat (word.unsigned len)) (List.map word.unsigned S) mod prime =
+                                       aval * bval * ri^(word.unsigned len) mod prime
+                                     )
+                                    )
+               )
+               lt _ _ _ _ _ _ _ _ _ _ _ _ _);
+        cbn [reconstruct map.putmany_of_list HList.tuple.to_list
+         HList.hlist.foralls HList.tuple.foralls
+         HList.hlist.existss HList.tuple.existss
+         HList.hlist.apply  HList.tuple.apply
+         HList.hlist
+         List.repeat Datatypes.length
+         HList.polymorphic_list.repeat HList.polymorphic_list.length
+         PrimitivePair.pair._1 PrimitivePair.pair._2] in *.
 
+          { repeat straightline. }
+          
+          { exact Wf_nat.lt_wf. }
+
+          { repeat straightline.
+            subst i i0. replace (word.add x1 (word.mul (word.of_Z 8) (word.of_Z 0))) with (x1) in H13 by ring. 
+            rewrite word.unsigned_of_Z_0 in H13. replace (word.unsigned x2 - 0) with (word.unsigned x2) in H13 by ring.
+            repeat split; eauto. 
+            - cbv [zeros]. rewrite repeat_length. rewrite H5. rewrite Nat2Z.id. trivial. 
+            - rewrite word.unsigned_of_Z_0.
+              
+              assert (eval_zero: forall beep boop,  @eval r beep (map word.unsigned (zeros boop)) = 0 ).
+              { clear; intros.
+                cbv [zeros eval Core.Positional.eval Core.Associational.eval Core.Positional.to_associational].
+                generalize dependent (map (UniformWeight.uweight r) (seq 0 beep)).
+                induction (Z.to_nat boop).
+                - simpl. destruct l; trivial.
+                - intros l'. cbn [repeat map]. rewrite word.unsigned_of_Z_0. destruct l'; trivial.
+                  cbn [combine map fst snd fold_right]. rewrite IHn. ring.
+              }
+
+              rewrite eval_zero.
+
+              assert (eval_in_name_only: forall xs, @eval r 0 xs = 0).
+              {  clear; intros.
+                cbv [eval Core.Positional.eval Core.Associational.eval Core.Positional.to_associational].
+                reflexivity.
+              }
+              rewrite eval_in_name_only. eexists.
+
+            - rewrite word.unsigned_of_Z_0. rewrite H5. apply Nat2Z.is_nonneg.
+              
+          }
+
+          { repeat straightline. eexists. split. { repeat straightline. } repeat straightline. split.
+
+            (*loop exits properly*)
+            2: {
+              repeat straightline; repeat split. exists x8; split; trivial.
+              destruct (word.ltu x16 x15) eqn: Hbreak.
+              - rewrite word.unsigned_of_Z_1 in H14; inversion H14.
+              - subst x5.  rewrite word.unsigned_ltu in Hbreak.
+                assert (word.unsigned x15 = word.unsigned x16) by Lia.lia.
+                rewrite H10 in *. apply H11.              
+            }
+
+            (*loop body good*)
+            repeat straightline.
+            eexists. repeat straightline.
+            
+        }
+
+          {  }
+          
+        }
+    Qed.
+    
+    Theorem redc_alt_ok :
+      program_logic_goal_for_function! redc_alt.
+    Proof.
+      repeat straightline.
+      (*after the first loop, our output array is full of zeros*)
+      refine ( tailrec (HList.polymorphic_list.cons _ (HList.polymorphic_list.cons _ (HList.polymorphic_list.cons _ (HList.polymorphic_list.cons _ (HList.polymorphic_list.cons _ (HList.polymorphic_list.cons _ (HList.polymorphic_list.cons _ (HList.polymorphic_list.cons _ HList.polymorphic_list.nil))))))))
+               ("Astart":: "Bstart" :: "Sstart" :: "len" :: "i" :: nil)
+               (fun l A aval B bval S Ra Rb R t m Astart Bstart Sstart len i => PrimitivePair.pair.mk
+                                    (m =* array scalar (word.of_Z 8) (word.add Sstart (word.mul (word.of_Z 8) i)) S * R /\
+                                       word.unsigned len - word.unsigned i = Z.of_nat (List.length S) /\
+                                       (*andres says i dont need this but im trying anyway*)
+                                       m =* array scalar (word.of_Z 8) (word.add Sstart (word.mul (word.of_Z 8) i)) A * Ra /\
+                                       m =* array scalar (word.of_Z 8) (word.add Sstart (word.mul (word.of_Z 8) i)) B * Rb /\
+                                       (* '\_O_/` *)
+
+                                       
+                                    l = List.length S ) 
+                                    (fun t' m' Astart' Bstart' Sstart' len' i' =>
+                                       (
+                                     t = t' /\ Astart = Astart' /\ Bstart = Bstart' /\ Sstart = Sstart' /\ len = len' /\
+                                     m' =* array scalar (word.of_Z 8) (word.add Sstart (word.mul (word.of_Z 8) i)) (zeros (word.unsigned len - word.unsigned i)) * R
+                                     )
+                                    )
+               )
+               lt _ _ _ _ _ _ _ _ _ _ _ _ _);
+        cbn [reconstruct map.putmany_of_list HList.tuple.to_list
+         HList.hlist.foralls HList.tuple.foralls
+         HList.hlist.existss HList.tuple.existss
+         HList.hlist.apply  HList.tuple.apply
+         HList.hlist
+         List.repeat Datatypes.length
+         HList.polymorphic_list.repeat HList.polymorphic_list.length
+         PrimitivePair.pair._1 PrimitivePair.pair._2] in *.
+      
+      { repeat straightline. }
+      { exact Wf_nat.lt_wf. }
+      { repeat straightline.
+        assert (Hwords: (word.add Sstart (word.mul (word.of_Z 8) i)) = Sstart).
+        { subst i. rewrite <-  word.ring_morph_mul. rewrite Z.mul_0_r.
+          assert (HstartZ: Sstart = word.of_Z (word.unsigned Sstart)) by (rewrite word.of_Z_unsigned; reflexivity).
+          rewrite HstartZ. rewrite <- word.ring_morph_add. rewrite Z.add_0_r. reflexivity.
+        }
+        rewrite Hwords. repeat split; try eauto. subst i. rewrite word.unsigned_of_Z_0. rewrite H5. ring. }
+
+      { repeat straightline. eexists. split. { repeat straightline. } repeat straightline. split.
+
+        (*loop exits properly*)
+        2: {
+          repeat straightline; repeat split.
+          rename x3 into S'; rename x9 into Sstart'; rename x10 into len'; rename x11 into i'; rename x6 into R'.
+
+          destruct (word.ltu i' len') eqn: Hbreak; try inversion H12; clear H12.
+          destruct (length S') eqn: HS.
+          (*length cannot be nonzero*)
+          2: { rewrite word.unsigned_ltu in Hbreak. Lia.lia. }
+          (*if length is zero, all arrays are the same*)
+          cbv [Z.of_nat] in H9. rewrite H9; clear H9 Hbreak.
+          apply ListUtil.length0_nil in HS.
+          subst S'. apply H8.
+        }
+          
+        (*loop body is good*)
+        repeat straightline.
+        rename x3 into S'; rename x9 into Sstart'; rename x10 into len'; rename x11 into i'; rename x6 into R'.
+        destruct S'.
+        - cbv [length Z.of_nat] in H9. 
+          destruct (word.ltu i' len') eqn: Hbreak; try (rewrite word.unsigned_of_Z_0 in H12; exfalso; apply H12; trivial).
+          rewrite word.unsigned_ltu in Hbreak. Lia.lia. 
+        - cbn [array] in H8. repeat straightline.
+          repeat split; try trivial. exists (S'). repeat split; try trivial. exists ( (scalar (word.add Sstart' (word.mul (word.of_Z 8) i')) (word.of_Z 0)) * R')%sep. exists (length S').
+          repeat split; subst v0 a.
+          all: try (repeat (destruct H12 as [solver H12]; try assumption; clear solver)).
+          + replace (word.mul (word.of_Z 8) i) with (word.add (word.mul (word.of_Z 8) i') (word.of_Z 8)).
+            { rewrite word.add_assoc. apply sep_comm. apply sep_assoc. ecancel_assumption. }
+            { subst i. ring. } 
+          + subst i. 
+            destruct (word.unsigned i' + 1 <? 2^64) eqn: Hisize.
+            2: { assert (2^64 - 1 <= word.unsigned i') by Lia.lia; clear Hisize.
+                 assert (word.unsigned i' < 2^64) by apply word.unsigned_range.
+                 assert (Hi': word.unsigned i' = 2^64 - 1) by Lia.lia; clear H12 H13.
+                 assert (Hlen': word.unsigned len' < 2^64) by apply word.unsigned_range.
+                 assert (Hneg: word.unsigned len' - word.unsigned i' < 1) by Lia.lia; clear Hi' Hlen'.
+                 simpl in H9; simpl in Hneg. rewrite Zpos_P_of_succ_nat in H9.
+                 assert (0 <= (Z.of_nat(length S'))) by apply Zle_0_nat.
+                 Lia.lia.
+            }
+                        
+            rewrite word.unsigned_add. rewrite word.unsigned_of_Z_1. cbv [word.wrap].
+            assert (Hsmall: (word.unsigned i' + 1) mod 2^64 = word.unsigned i' + 1).
+            {  apply Z.mod_small. assert (0 <= word.unsigned i') by apply word.unsigned_range. Lia.lia. }
+            rewrite Hsmall; clear Hisize Hsmall.
+
+            simpl in H9; simpl. rewrite Zpos_P_of_succ_nat in H9.
+            assert (0 <= (Z.of_nat(length S'))) by apply Zle_0_nat.
+            Lia.lia.
+          + subst v.  auto.
+          + assert (Hhead: zeros (word.unsigned len' - word.unsigned i') = word.of_Z 0 :: zeros (word.unsigned len' - word.unsigned i) ).
+            {
+              subst i. 
+            destruct (word.unsigned i' + 1 <? 2^64) eqn: Hisize.
+            2: { assert (2^64 - 1 <= word.unsigned i') by Lia.lia; clear Hisize.
+                 assert (word.unsigned i' < 2^64) by apply word.unsigned_range.
+                 assert (Hi': word.unsigned i' = 2^64 - 1) by Lia.lia; clear H12 H13.
+                 assert (Hlen': word.unsigned len' < 2^64) by apply word.unsigned_range.
+                 assert (Hneg: word.unsigned len' - word.unsigned i' < 1) by Lia.lia; clear Hi' Hlen'.
+                 simpl in H9; simpl in Hneg. rewrite Zpos_P_of_succ_nat in H9.
+                 assert (0 <= (Z.of_nat(length S'))) by apply Zle_0_nat.
+                 Lia.lia.
+            }
+                        
+            rewrite word.unsigned_add. rewrite word.unsigned_of_Z_1. cbv [word.wrap].
+            assert (Hsmall: (word.unsigned i' + 1) mod 2^64 = word.unsigned i' + 1).
+            {  apply Z.mod_small. assert (0 <= word.unsigned i') by apply word.unsigned_range. Lia.lia. }
+            rewrite Hsmall; clear Hisize Hsmall.
+            assert (Hpos: 0 <= word.unsigned len' - (word.unsigned i' + 1)). {
+              simpl in H9; simpl. rewrite Zpos_P_of_succ_nat in H9.
+              assert (0 <= (Z.of_nat(length S'))) by apply Zle_0_nat.
+              Lia.lia.
+            }
+            replace (word.unsigned len' - word.unsigned i') with (Z.succ (word.unsigned len' - (word.unsigned i' + 1)) ) by Lia.lia.
+            cbv [zeros]. rewrite Z2Nat.inj_succ; try assumption. cbn [repeat]. trivial.
+            }
+            rewrite Hhead; clear Hhead.
+            cbn [array]. subst i. 
+            replace (word.add (word.add Sstart' (word.mul (word.of_Z 8) i')) (word.of_Z 8)) with  (word.add Sstart' (word.mul (word.of_Z 8) (word.add i' (word.of_Z 1)))) by ring. ecancel_assumption.
+        }
+     
+        {
+          repeat straightline.
+          
+          refine ( tailrec (HList.polymorphic_list.cons _ (HList.polymorphic_list.cons _ (HList.polymorphic_list.cons _ (HList.polymorphic_list.cons _ (HList.polymorphic_list.cons _ (HList.polymorphic_list.cons _ (HList.polymorphic_list.cons _ (HList.polymorphic_list.cons _ HList.polymorphic_list.nil))))))))
+               ("Astart":: "Bstart" :: "Sstart" :: "len" :: "i" :: nil)
+               (fun l A aval B bval S Ra Rb R t m Astart Bstart Sstart len i => PrimitivePair.pair.mk
+                                            (m =* array scalar (word.of_Z 8) Astart A * Ra /\
+                                            m =* array scalar (word.of_Z 8) Bstart B * Rb /\
+                                            m =* array scalar (word.of_Z 8) Sstart S * R /\
+                                            word.unsigned len = Z.of_nat (List.length A)  /\
+                                            word.unsigned len = Z.of_nat (List.length B)  /\
+                                            word.unsigned len = Z.of_nat (List.length S) /\
+                                            @eval r (Z.to_nat (word.unsigned len)) (List.map word.unsigned A) = aval /\ 
+                                            @eval r (Z.to_nat (word.unsigned len)) (List.map word.unsigned B) = bval /\
+                                            @eval r (Z.to_nat (word.unsigned len)) (List.map word.unsigned S) mod prime =
+                                            @eval (word.unsigned i) (Z.to_nat (word.unsigned len)) (List.map word.unsigned A) * bval * ri^(word.unsigned i) /\
+                                            l = Z.to_nat (word.unsigned len - word.unsigned i) )
+                                    (fun t' m' Astart' Bstart' Sstart' len' i' =>
+                                     (
+                                     t = t' /\ Astart = Astart' /\ Bstart = Bstart' /\ Sstart = Sstart' /\ len = len' /\
+                                     exists S',
+                                       m' =* array scalar (word.of_Z 8) Sstart S' * R /\
+                                       @eval r (Z.to_nat (word.unsigned len)) (List.map word.unsigned S) mod prime =
+                                       aval * bval * ri^(word.unsigned len)
+                                     )
+                                    )
+               )
+               lt _ _ _ _ _ _ _ _ _ _ _ _ _);
+        cbn [reconstruct map.putmany_of_list HList.tuple.to_list
+         HList.hlist.foralls HList.tuple.foralls
+         HList.hlist.existss HList.tuple.existss
+         HList.hlist.apply  HList.tuple.apply
+         HList.hlist
+         List.repeat Datatypes.length
+         HList.polymorphic_list.repeat HList.polymorphic_list.length
+         PrimitivePair.pair._1 PrimitivePair.pair._2] in *.
+
+          { repeat straightline. }
+          
+          { exact Wf_nat.lt_wf. }
+
+          { repeat straightline.
+            repeat split.
+            - 
+            -
+            -
+            -
+            -
+            -
+            -
+              
+              
+          }
+
+          {  }
+
+          {  }
+          
+        }
+    Qed.
+    
+ 
+    
     End WithParameters.
